theories/SepCreditsNew.v
@@ -1,61 +1,1209 @@
+(**
+
+This file formalizes Separation Logic with possibly negative
+time credits. It is described in the paper:
+
+"Formal Proof and Analysis of an Incremental Cycle Detection Algorithm"
+(ITP'19)
+
+It is a variant of the Separation Logic with time credits in [nat],
+described in the papers:
+
+- Machine-Checked Verification of the Correctness and Amortized
+  Complexity of an Efficient Union-Find Implementation (ITP'15)
+
+- Verifying the Correctness and Amortized Complexity of a Union-Find
+  Implementation in Separation Logic with Time Credits (JAR'17)
+
+This file contains:
+- a definition of heaps as finite maps from location to values
+  paired with a natural number,
+- an instantiation of the functor from the file SepFunctor.v,
+- a definition of triples,
+- statement and proofs of SL reasoning rules.
+
+Author: Arthur Charguéraud.
+License: CC-by 4.0.
+
+*)
+
+Set Implicit Arguments.
+From Sep Require Export Semantics SepFunctor.
+From Sep Require Import Fmap.
+Open Scope fmap_scope.
+
+
+
+(* ********************************************************************** *)
+(* * Semantics *)
+
+(* ---------------------------------------------------------------------- *)
+(* ** Big-step evaluation with counting of the number of beta reductions
+    (used by the formalization of Separation Logic with time credits) *)
+
+Section Redn.
+Local Open Scope nat_scope.
+Local Open Scope fmap_scope.
+
+Implicit Types t : trm.
+Implicit Types v : val.
+Implicit Types b : bool.
+
+Inductive eval : nat -> state -> trm -> state -> val -> Prop :=
+  | eval_val : forall m v,
+      eval 0 m (trm_val v) m v
+  | eval_fix : forall m f x t1,
+      eval 0 m (trm_fix f x t1) m (val_fix f x t1)
+  | eval_if : forall n m1 m2 b r t1 t2,
+      eval m1 n (if b then t1 else t2) m2 r ->
+      eval m1 n (trm_if (val_bool b) t1 t2) m2 r
+  | eval_let : forall n1 n2 m1 m2 m3 z t1 t2 v1 r,
+      eval n1 m1 t1 m2 v1 ->
+      eval n2 m2 (subst1 z v1 t2) m3 r ->
+      eval (n1+n2) m1 (trm_let z t1 t2) m3 r
+  | eval_app_arg : forall n1 n2 n3 m1 m2 m3 m4 t1 t2 v1 v2 f x t r,
+      eval n1 m1 t1 m2 v1 ->
+      eval n2 m2 t2 m3 v2 ->
+      v1 = val_fix f x t ->
+      eval n3 m3 (subst2 f v1 x v2 t) m4 r ->
+      eval (n1+n2+n3+1) m1 (trm_app t1 t2) m4 r
+  | eval_ref : forall m v l,
+      ~ Fmap.indom m l ->
+      l <> null ->
+      eval 0 m (val_ref v) (Fmap.update m l v) (val_loc l)
+  | eval_get : forall m l,
+      Fmap.indom m l ->
+      eval 0 m (val_get (val_loc l)) m (Fmap.read m l)
+  | eval_set : forall m l v,
+      Fmap.indom m l ->
+      eval 0 m (val_set (val_loc l) v) (Fmap.update m l v) val_unit
+  | eval_free : forall m l,
+      Fmap.indom m l ->
+      eval 0 m (val_free (val_loc l)) (Fmap.remove m l) val_unit.
+
+Hint Resolve eval_val.
+
+Lemma eval_app_fix_val : forall n m1 m2 v1 v2 f x t r,
+  v1 = val_fix f x t ->
+  eval n m1 (subst2 f v1 x v2 t) m2 r ->
+  eval (n+1) m1 (trm_app v1 v2) m2 r.
+Proof using.
+  introv E M. subst. applys_eq* eval_app_arg. math.
+Qed.
+
+Lemma eval_ref_sep : forall s1 s2 v l,
+  l <> null ->
+  s2 = Fmap.single l v ->
+  Fmap.disjoint s2 s1 ->
+  eval 0 s1 (val_ref v) (Fmap.union s2 s1) (val_loc l).
+Proof using.
+  introv Nl -> D. forwards Dv: Fmap.indom_single l v.
+  rewrite <- Fmap.update_eq_union_single. applys~ eval_ref.
+  { intros N. applys~ Fmap.disjoint_inv_not_indom_both D N. }
+Qed.
+
+Lemma eval_get_sep : forall s s1 s2 l v,
+  s = Fmap.union s1 s2 ->
+  Fmap.disjoint s1 s2 ->
+  s1 = Fmap.single l v ->
+  eval 0 s (val_get (val_loc l)) s v.
+Proof using.
+  introv -> D ->. forwards Dv: Fmap.indom_single l v.
+  applys_eq eval_get.
+  { rewrite~ Fmap.read_union_l. rewrite~ Fmap.read_single. }
+  { applys~ Fmap.indom_union_l. }
+Qed.
+
+Lemma eval_set_sep : forall s s' h1 h1' h2 l v v',
+  s = Fmap.union h1 h2 ->
+  s' = Fmap.union h1' h2 ->
+  Fmap.disjoint h1 h2 ->
+  h1 = Fmap.single l v ->
+  h1' = Fmap.single l v' ->
+  eval 0 s (val_set (val_loc l) v') s' val_unit.
+Proof using.
+  introv -> -> D -> ->. forwards Dv: Fmap.indom_single l v.
+  applys_eq eval_set.
+  { rewrite~ Fmap.update_union_l. fequals.
+    rewrite~ Fmap.update_single. }
+  { applys~ Fmap.indom_union_l. }
+Qed.
+
+Lemma eval_free_sep : forall s1 s2 v l,
+  s1 = Fmap.union (Fmap.single l v) s2 ->
+  Fmap.disjoint (Fmap.single l v) s2 ->
+  eval 0 s1 (val_free l) s2 val_unit.
+Proof using.
+  introv -> D. forwards Dv: Fmap.indom_single l v.
+  applys_eq eval_free.
+  { rewrite~ Fmap.remove_union_single_l.
+    intros Dl. applys Fmap.disjoint_inv_not_indom_both D Dl.
+    applys Fmap.indom_single. }
+  { applys~ Fmap.indom_union_l. }
+Qed.
+
+End Redn.
+
+
+
+(* ********************************************************************** *)
+(* * Core of the logic *)
+
+Module Export SepCreditsCore <: SepCore.
+
+
+(* ---------------------------------------------------------------------- *)
+(* ** Representation of credits *)
+
+(** Representation of credits *)
+
+Definition credits : Type := int.
+
+(** Hint for [math] tactic to unfold [credits] definition *)
+
+Ltac math_0 ::= unfolds credits.
+
+(** Zero and one credits *)
+
+Definition credits_zero : credits := 0.
+
+Definition credits_one : credits := 1.
+
+
+(* ---------------------------------------------------------------------- *)
+(** Heaps *)
+
+Declare Scope heap_scope.
+
+(** Type of heaps *)
+
+Definition heap : Type := (state * credits)%type.
+
+(** Empty heap *)
+
+Definition heap_empty : heap :=
+  (Fmap.empty, 0).
+
+(** Projections *)
+
+Definition heap_state (h:heap) : state :=
+  match h with (m,c) => m end.
+
+Definition heap_credits (h:heap) : credits :=
+  match h with (m,c) => c end.
+
+Notation "h '^s'" := (heap_state h)
+   (at level 9, format "h '^s'") : heap_scope.
+
+Notation "h '^c'" := (heap_credits h)
+   (at level 9, format "h '^c'") : heap_scope.
+
+Open Scope heap_scope.
+
+(** Disjoint heaps *)
+
+Definition heap_disjoint (h1 h2 : heap) : Prop :=
+  Fmap.disjoint (h1^s) (h2^s).
+
+Notation "\# h1 h2" := (heap_disjoint h1 h2)
+  (at level 40, h1 at level 0, h2 at level 0, no associativity) : heap_scope.
+
+(** Union of heaps *)
+
+Definition heap_union (h1 h2 : heap) : heap :=
+   (h1^s \+ h2^s, h1^c + h2^c).
+
+Declare Scope heap_union_scope.
+
+Notation "h1 \u h2" := (heap_union h1 h2)
+   (at level 37, right associativity) : heap_union_scope.
+
+Local Open Scope heap_union_scope.
+
+(** Affine heaps are those such that [heap_credits c >= 0] *)
+
+Definition heap_affine (h:heap) : Prop :=
+  h^c >= 0.
+
+(** Properties of [heap_affine] *)
+
+Lemma heap_affine_heap_empty :
+  heap_affine heap_empty.
+Proof using.
+  unfold heap_affine, heap_empty. simpl. math.
+Qed.
+
+Lemma heap_affine_heap_union : forall h1 h2,
+  heap_affine h1 ->
+  heap_affine h2 ->
+  heap_affine (h1 \u h2).
+Proof using.
+  intros [m1 n1] [m2 n2] M1 M2. unfolds heap_affine, heap_union.
+  simpls. math.
+Qed.
+
+
+(* ---------------------------------------------------------------------- *)
+(* ** Hprop *)
+
+(** A heap predicate, type [hprop] is a predicate over such heaps. *)
+
+Definition hprop := heap -> Prop.
+
+
+(* ---------------------------------------------------------------------- *)
+(* ** Entailment *)
+
+Definition himpl (H1 H2:hprop) : Prop :=
+  forall (h:heap), H1 h -> H2 h.
+
+Notation "H1 ==> H2" := (himpl H1 H2) (at level 55) : heap_scope.
+
+Local Open Scope heap_scope.
+
+Definition qimpl A (Q1 Q2:A->hprop) : Prop :=
+  forall (v:A), Q1 v ==> Q2 v.
+
+Notation "Q1 ===> Q2" := (qimpl Q1 Q2) (at level 55) : heap_scope.
+
+Lemma himpl_refl : forall H,
+  H ==> H.
+Proof using. introv M. auto. Qed.
+
+Lemma himpl_trans : forall H2 H1 H3,
+  (H1 ==> H2) ->
+  (H2 ==> H3) ->
+  (H1 ==> H3).
+Proof using. introv M1 M2. intros h H1h. eauto. Qed.
+
+Lemma himpl_antisym : forall H1 H2,
+  (H1 ==> H2) ->
+  (H2 ==> H1) ->
+  (H1 = H2).
+Proof using. introv M1 M2. applys pred_ext_1. intros h. iff*. Qed.
+
+
+(* ---------------------------------------------------------------------- *)
+(** Operators *)
+
+(** Affinity is defined in the standard way *)
+
+Definition haffine (H : hprop) : Prop :=
+  forall h, H h -> heap_affine h.
+
+(** Heap predicates *)
+
+Definition hempty : hprop :=
+  fun h => h = heap_empty.
+
+Definition hstar (H1 H2 : hprop) : hprop :=
+  fun h => exists h1 h2,
+              H1 h1
+           /\ H2 h2
+           /\ heap_disjoint h1 h2
+           /\ h = h1 \u h2.
+
+Definition hexists A (J : A -> hprop) : hprop :=
+  fun h => exists x, J x h.
+
+Definition hforall A (J : A -> hprop) : hprop :=
+  fun h => forall x, J x h.
+
+(** Notation *)
+
+Notation "\[]" := (hempty)
+  (at level 0) : heap_scope.
+
+Notation "H1 '\*' H2" := (hstar H1 H2)
+  (at level 41, right associativity) : heap_scope.
+
+Notation "Q \*+ H" := (fun x => hstar (Q x) H)
+  (at level 40) : heap_scope.
+
+
+(* ---------------------------------------------------------------------- *)
+(* ** Types *)
+
+Implicit Types H : hprop.
+Implicit Types Q : val->hprop.
+
+
+(* ---------------------------------------------------------------------- *)
+(* ** Tactic for automation *)
+
+Hint Extern 1 (_ = _ :> heap) => fmap_eq.
+
+Lemma heap_disjoint_def : forall h1 h2,
+  heap_disjoint h1 h2 = Fmap.disjoint (h1^s) (h2^s).
+Proof using. auto. Qed.
+
+Hint Rewrite heap_disjoint_def : rew_disjoint.
+
+Tactic Notation "fmap_disjoint_pre" :=
+  subst; rew_disjoint; jauto_set.
+
+Hint Extern 1 (heap_disjoint _ _) => fmap_disjoint_pre.
+
+
+(* ---------------------------------------------------------------------- *)
+(* ** Equalities on [heap] *)
+
+Lemma heap_eq : forall h1 h2,
+  (h1^s = h2^s /\ h1^c = h2^c) -> h1 = h2.
+Proof using.
+  intros (s1,n1) (s2,n2) (M1&M2). simpls. subst. fequals.
+Qed.
+
+Lemma heap_eq_forward : forall h1 h2,
+  h1 = h2 ->
+  h1^s = h2^s /\ h1^c = h2^c.
+Proof using. intros (s1,n1) (s2,n2) M. inverts~ M. Qed.
+
+
+(* ---------------------------------------------------------------------- *)
+(* ** Properties of [heap_disjoint] *)
+
+Lemma heap_disjoint_sym : forall h1 h2,
+  \# h1 h2 -> \# h2 h1.
+Proof using.
+  intros [m1 n1] [m2 n2] H. simpls.
+  hint Fmap.disjoint_sym. autos*.
+Qed.
+
+Lemma heap_disjoint_comm : forall h1 h2,
+  \# h1 h2 = \# h2 h1.
+Proof using.
+  intros [m1 n1] [m2 n2]. simpls.
+  hint heap_disjoint_sym. extens*.
+Qed.
+
+Lemma heap_disjoint_empty_l : forall h,
+  \# heap_empty h.
+Proof using. intros [m n]. hint Fmap.disjoint_empty_l. hnfs*. Qed.
+
+Lemma heap_disjoint_empty_r : forall h,
+  \# h heap_empty.
+Proof using. intros [m n]. hint Fmap.disjoint_empty_r. hnfs*. Qed.
+
+Lemma heap_disjoint_union_eq_r : forall h1 h2 h3,
+  \# h1 (h2 \u h3) = (\# h1 h2 /\ \# h1 h3).
+Proof using.
+  intros [m1 n1] [m2 n2] [m3 n3].
+  unfolds heap_disjoint, heap_union. simpls.
+  rewrite Fmap.disjoint_union_eq_r. extens*.
+Qed.
+
+Lemma heap_disjoint_union_eq_l : forall h1 h2 h3,
+  \# (h2 \u h3) h1 = (\# h1 h2 /\ \# h1 h3).
+Proof using.
+  intros. rewrite heap_disjoint_comm.
+  apply heap_disjoint_union_eq_r.
+Qed.
+
+Hint Resolve
+   heap_disjoint_sym
+   heap_disjoint_empty_l heap_disjoint_empty_r
+   heap_disjoint_union_eq_l heap_disjoint_union_eq_r.
+
+Tactic Notation "rew_disjoint" :=
+  autorewrite with rew_disjoint in *.
+Tactic Notation "rew_disjoint" "*" :=
+  rew_disjoint; auto_star.
+
+
+(* ---------------------------------------------------------------------- *)
+(* ** Properties of [heap_union] *)
+
+Lemma heap_union_comm : forall h1 h2,
+  \# h1 h2 ->
+  h1 \u h2 = h2 \u h1.
+Proof using.
+  intros [m1 n1] [m2 n2] H. unfold heap_union.
+  simpl. fequals. fmap_eq. math.
+Qed.
+
+Lemma heap_union_assoc : forall h1 h2 h3,
+  (h1 \u h2) \u h3 = h1 \u (h2 \u h3).
+Proof using.
+  intros [m1 n1] [m2 n2] [m3 n3]. unfolds heap_union.
+  simpl. fequals. fmap_eq. math.
+Qed.
+
+Lemma heap_union_empty_l : forall h,
+  heap_empty \u h = h.
+Proof using.
+  intros [m n]. unfold heap_union, heap_empty. simpl.
+  fequals. apply~ Fmap.union_empty_l.
+Qed.
+
+Lemma heap_union_empty_r : forall h,
+  h \u heap_empty = h.
+Proof using.
+  intros. rewrite~ heap_union_comm. apply~ heap_union_empty_l.
+Qed.
+
+Lemma heap_union_state : forall h1 h2,
+  heap_state (h1 \u h2) = (heap_state h1) \+ (heap_state h2).
+Proof using. intros (m1&n1) (m2&n2). auto. Qed.
+
+Lemma heap_union_credits : forall h1 h2,
+  heap_credits (h1 \u h2) = (heap_credits h1 + heap_credits h2).
+Proof using. intros (m1&n1) (m2&n2). auto. Qed.
+
+Hint Resolve heap_union_comm
+   heap_union_empty_l heap_union_empty_r.
+
+Hint Rewrite heap_union_state : rew_disjoint.
+
+(* Extend the tactic [fmap_eq] with distribution of [heap_state] *)
+Hint Rewrite heap_union_state : rew_fmap_for_fmap_eq.
+
+Hint Rewrite
+  heap_union_empty_l heap_union_empty_r
+  heap_union_state heap_union_credits : rew_heap.
+
+Tactic Notation "rew_heap" :=
+  autorewrite with rew_heap.
+Tactic Notation "rew_heap" "~" :=
+  rew_heap; auto_tilde.
+Tactic Notation "rew_heap" "in" hyp(H) :=
+  autorewrite with rew_heap in H.
+Tactic Notation "rew_heap" "~" "in" hyp(H) :=
+  rew_heap in H; auto_tilde.
+Tactic Notation "rew_heap" "in" "*" :=
+  autorewrite with rew_heap in *.
+Tactic Notation "rew_heap" "~" "in" "*" :=
+  rew_heap in *; auto_tilde.
+
+Ltac heap_eq :=
+  solve [ rew_heap; subst; auto ].
+
+
+(* ---------------------------------------------------------------------- *)
+(* ** Properties of empty *)
+
+Lemma hempty_intro :
+  \[] heap_empty.
+Proof using. hnfs~. Qed.
+
+Lemma hempty_inv : forall h,
+  \[] h ->
+  h = heap_empty.
+Proof using. auto. Qed.
+
+
+(* ---------------------------------------------------------------------- *)
+(* ** Core properties *)
+
+Section Properties.
+
+Hint Resolve hempty_intro.
+
+Lemma hstar_hempty_l : forall H,
+  hempty \* H = H.
+Proof using.
+  intros. applys pred_ext_1. intros h.
+  iff (h1&h2&M1&M2&D&U) M.
+  { forwards E: hempty_inv M1. subst.
+    rewrite~ heap_union_empty_l. }
+  { exists~ heap_empty h. }
+Qed.
+
+Lemma hstar_comm : forall H1 H2,
+   H1 \* H2 = H2 \* H1.
+Proof using.
+  intros H1 H2. unfold hprop, hstar. extens. intros h.
+  iff (h1&h2&M1&M2&D&U); rewrite~ heap_union_comm in U; exists* h2 h1.
+Qed.
+
+Lemma hstar_assoc : forall H1 H2 H3,
+  (H1 \* H2) \* H3 = H1 \* (H2 \* H3).
+Proof using.
+  intros H1 H2 H3. unfold hprop, hstar. extens. intros h. split.
+  { intros (h'&h3&(h1&h2&M3&M4&D'&U')&M2&D&U). subst h'.
+    exists h1 (h2 \u h3). splits~.
+    { exists h2 h3. splits*. }
+    { subst. applys heap_eq. split. { fmap_eq. } { simpl; math. } } }
+  { intros (h1&h'&M1&(h2&h3&M3&M4&D'&U')&D&U). subst h'.
+    exists (h1 \u h2) h3. splits~.
+    { exists h1 h2. splits*. }
+    { subst. applys heap_eq. split. { fmap_eq. } { simpl; math. } } }
+Qed.
+
+Lemma hstar_hexists : forall A (J:A->hprop) H,
+  (hexists J) \* H = hexists (fun x => (J x) \* H).
+Proof using.
+  intros. applys pred_ext_1. intros h. iff M.
+  { destruct M as (h1&h2&(x&M1)&M2&D&U). exists~ x h1 h2. }
+  { destruct M as (x&(h1&h2&M1&M2&D&U)). exists h1 h2. splits~. exists~ x. }
+Qed.
+
+Lemma hstar_hforall : forall H A (J:A->hprop),
+  (hforall J) \* H ==> hforall (J \*+ H).
+Proof using.
+  intros. intros h M. destruct M as (h1&h2&M1&M2&D&U). intros x. exists~ h1 h2.
+Qed.
+
+Lemma himpl_frame_l : forall H2 H1 H1',
+  H1 ==> H1' ->
+  (H1 \* H2) ==> (H1' \* H2).
+Proof using. introv W (h1&h2&?). exists* h1 h2. Qed.
+
+Lemma haffine_hempty :
+  haffine \[].
+Proof using.
+  introv M. lets ->: hempty_inv M. applys heap_affine_heap_empty.
+Qed.
+
+Lemma haffine_hstar : forall H1 H2,
+  haffine H1 ->
+  haffine H2 ->
+  haffine (H1 \* H2).
+Proof using.
+  introv F1 F2 (h1&h2&M1&M2&D&->). applys* heap_affine_heap_union.
+Qed.
+
+End Properties.
+
+End SepCreditsCore.
+
+
+
+(* ********************************************************************** *)
+(* * Derived properties of the logic *)
+
+(** Here, we instantiate the functors to obtained derived definitions,
+  lemmas, notation, and tactics. *)
+
+Module Export SepCreditsSetup := SepSetup SepCreditsCore.
+Export SepCreditsCore.
+
+Local Open Scope heap_union_scope.
+
+Implicit Types H : hprop.
+Implicit Types Q : val->hprop.
+Implicit Types P : Prop.
+
+(* ********************************************************************** *)
+(* * Specific properties of the logic *)
+
+
+(* ---------------------------------------------------------------------- *)
+(* ** Auxiliary lemmas *)
+
+Section Aux.
+
+Lemma hpure_inv : forall P h,
+  \[P] h ->
+  P /\ h = heap_empty.
+Proof using.
+  introv M. lets (HP&HE): hpure_inv_hempty M.
+  lets*: hempty_inv HE.
+Qed.
+
+Lemma hpure_intro : forall P,
+  P ->
+  \[P] heap_empty.
+Proof using. introv M. applys~ hpure_intro_hempty. applys hempty_intro. Qed.
+
+Lemma hstar_intro : forall H1 H2 h1 h2,
+  H1 h1 ->
+  H2 h2 ->
+  heap_disjoint h1 h2 ->
+  (H1 \* H2) (h1 \u h2).
+Proof using. intros. exists~ h1 h2. Qed.
+
+Lemma hstar_inv : forall H1 H2 h,
+  (H1 \* H2) h ->
+  exists h1 h2, H1 h1 /\ H2 h2 /\ heap_disjoint h1 h2 /\ h = h1 \u h2.
+Proof using. introv M. hnf in M. eauto. Qed.
+
+End Aux.
+
+
+(* ---------------------------------------------------------------------- *)
+(* ** Singleton heap *)
+
+Definition hsingle (l:loc) (v:val) : hprop :=
+  fun h => h^s = Fmap.single l v /\ h^c = credits_zero /\ l <> null.
+
+Notation "l '~~~>' v" := (hsingle l v)
+  (at level 32, no associativity) : heap_scope.
+Notation "l '~~>' v" := (hsingle l v)
+  (at level 32, no associativity) : heap_scope.
+
+Lemma hsingle_intro : forall l v,
+  l <> null ->
+  (l ~~~> v) ((Fmap.single l v), credits_zero).
+Proof using. intros. split~. Qed.
+
+Lemma hsingle_inv : forall h l v,
+  (l ~~~> v) h ->
+  h = (Fmap.single l v, credits_zero) /\ (l <> null).
+Proof using. intros (s,n) l v (E1&E2&N). simpls*. Qed.
+
+Lemma hstar_hsingle_same_loc : forall (l:loc) (v1 v2:val),
+  (l ~~~> v1) \* (l ~~~> v2) ==> \[False].
+Proof using.
+  intros. unfold hsingle.
+  intros h ((m1&n1)&(m2&n2)&(E1&X1&N1)&(E2&X2&N2)&D&E). false.
+  subst. applys* Fmap.disjoint_single_single_same_inv l v1 v2.
+  unfolds in D. rewrite <- E1. rewrite <- E2. auto.
+Qed.
+
+Arguments hstar_hsingle_same_loc : clear implicits.
+
+Lemma haffine_hsingle : forall l v,
+  haffine (hsingle l v).
+Proof using.
+  intros. rewrite haffine_eq.
+  introv (E&Ec&_). unfold heap_affine. rewrite Ec.
+  unfold credits_zero. math.
+Qed.
+
+Global Opaque hsingle.
+
+(* ** Configure [hcancel] to make it aware of [hsingle] *)
+
+(* not needed? *)
+Ltac xsimpl_hook H ::=
+  match H with
+  | hsingle _ _ => xsimpl_cancel_same H
+  end.
+
+Global Opaque hsingle.
+
+
+(* ---------------------------------------------------------------------- *)
+(* ** Credits heap *)
+
+Definition mk_heap_credits (n:credits) : heap :=
+  (Fmap.empty:state, n).
+
+Definition hcredits (n:credits) : hprop :=
+  fun h => h = mk_heap_credits n.
+
+Notation "'\$' n" := (hcredits n)
+  (at level 40, format "\$ n") : heap_scope.
+
+Lemma heap_credit_mk_heap_credits : forall n,
+  (mk_heap_credits n)^c = n.
+Proof using. auto. Qed.
+
+Hint Rewrite heap_credit_mk_heap_credits : rew_heap.
+
+Lemma hcredits_mk_heap_credits : forall n,
+  (\$n) (mk_heap_credits n).
+Proof using. intros. unfolds* hcredits. Qed.
+
+Lemma hcredits_inv : forall n h,
+  (\$n) h ->
+  h^s = Fmap.empty /\ h^c = n.
+Proof using.
+  introv N. unfolds hcredits, mk_heap_credits. subst*.
+Qed.
+
+Lemma haffine_hcredits : forall n,
+  n >= 0 ->
+  haffine (\$ n).
+Proof using.
+  introv N. rewrite haffine_eq. introv Hh.
+  lets (Hs&Hc): hcredits_inv Hh. unfold heap_affine. rewrite* Hc.
+Qed.
+
+Global Opaque hcredits.
+
+
+(* ---------------------------------------------------------------------- *)
+(* ** Affinity *)
+
+Section Affine.
+Transparent haffine.
+
+Lemma hgc_intro : forall h,
+  h^c >= 0 ->
+  \GC h.
+Proof using. introv N. applys* hgc_of_heap_affine. Qed.
+
+Lemma haffine_heap_inv : forall H h,
+  haffine H ->
+  H h ->
+  h^c >= 0.
+Proof using. introv F M. applys F M. Qed.
+
+Lemma hgc_heap_inv : forall h,
+  \GC h ->
+  h^c >= 0.
+Proof using. introv N. applys* haffine_heap_inv. applys haffine_hgc. Qed.
+
+End Affine.
+
+Global Opaque heap_affine.
+
+
+(* ---------------------------------------------------------------------- *)
+(* ** Properties of credits *)
+
+Section Credits.
+Transparent hcredits hempty hpure hstar mk_heap_credits heap_union heap_disjoint.
+
+Lemma hcredits_zero_eq : \$ 0 = \[].
+Proof using.
+  unfold hcredits, hempty, heap_empty.
+  applys pred_ext_1. intros [m n]; simpl. unfold mk_heap_credits. iff*.
+Qed.
+
+Lemma hcredits_add_eq : forall n m,
+  \$ (n+m) = \$ n \* \$ m.
+Proof using.
+  intros c1 c2. unfold hcredits, hstar, heap_union, heap_disjoint, mk_heap_credits.
+  applys pred_ext_1. intros [m n]. iff M.
+  { inverts M. exists___. splits*; simpl; try fmap_eq.
+    { fequals. fmap_eq. math. } }
+  { destruct M as ([m1 n1]&[m2 n2]&M3&M4&M5&M6).
+    inverts M3. inverts M4. rewrite M6. simpl. fequals. fmap_eq. }
+Qed.
+
+Lemma hcredits_sub : forall n m,
+  (n >= m) ->
+  \$ n ==> \$ m \* \$ (n-m).
+Proof using.
+  introv M. rewrite <- hcredits_add_eq.
+  math_rewrite (m + (n-m) = n). auto.
+Qed.
+
+Lemma hcredits_drop : forall n m,
+  n >= m ->
+  exists H', haffine H' /\ \$ n ==> \$ m \* H'.
+Proof using.
+  introv M. exists (\$(n-m)). split.
+  { apply haffine_hcredits. math. }
+  { applys* hcredits_sub. }
+Qed.
+
+End Credits.
+
+
+
+(* ********************************************************************** *)
+(* * Reasoning Rules *)
+
+Implicit Types t : trm.
+Implicit Types v w : val.
+Implicit Types h : heap.
+Implicit Types p : loc.
+
+
+(* ---------------------------------------------------------------------- *)
+(* ** Definitions of [pay] *)
+
+Definition pay_one H H' :=
+  H ==> (\$ 1) \* H'.
+
+
+(* ---------------------------------------------------------------------- *)
+(* ** Definition of Hoare triples *)
 
 
 Definition hoare (t:trm) (H:hprop) (Q:val->hprop) :=
-  forall h, H h -> exists h' v, eval (heap_state h) t (heap_state h') v
-                             /\ Q v h'
-
-Definition triple (t:trm) (H:hprop) (Q:val->hprop) : Prop :=
-  forall H', hoare t (H \* H') (Q \*+ H' \*+ \GC).
-
-
---------------
-heap = (state * Z)
-
-Definition hoare (t:trm) (H:hprop) (Q:val->hprop) :=
-  forall h, H h -> exists h' v, evaln n (heap_state h) t (heap_state h') v
+  forall h, H h -> exists n h' v, eval n (heap_state h) t (heap_state h') v
                              /\ Q v h'
                              /\ heap_credits h = n + heap_credits h'.
 
+(* ---------------------------------------------------------------------- *)
+(* ** Hoare rules *)
+
+Lemma hoare_conseq : forall t H' Q' H Q,
+  hoare t H' Q' ->
+  H ==> H' ->
+  Q' ===> Q ->
+  hoare t H Q.
+Proof using.
+  introv M MH MQ HF. forwards (n&h'&v&R&K&S): M h.
+  { applys* MH. }
+  exists n h' v. splits~. { applys MQ K. }
+Qed.
+
+Lemma hoare_val : forall H' v,
+  hoare (trm_val v) H' (fun r => \[r = v] \* H').
+Proof using.
+  introv. intros h K. exists 0%nat h v. splits~.
+  { applys eval_val. }
+  { rewrite* hstar_hpure_l. }
+Qed.
+
+Lemma hoare_fix : forall H' f x t1,
+  hoare (trm_fix f x t1) H' (fun r => \[r = (val_fix f x t1)] \* H').
+Proof using.
+  introv. intros h K. exists 0%nat h (val_fix f x t1). splits~.
+  { applys eval_fix. }
+  { rewrite* hstar_hpure_l. }
+Qed.
+
+Lemma pay_one_elim : forall H H' h,
+  pay_one H H' ->
+  H h -> 
+  exists h', H' h' /\ h = (mk_heap_credits 1 \u h').
+Proof using.
+  introv HP N. lets N': (rm HP) (rm N). rew_heap in N'.
+  destruct N' as (h1&h2&N1&N2&N3&N4).
+  lets (N1'&N2'): hcredits_inv (rm N1).
+  destruct h1 as [n1 c1]. simpls. subst*.
+Qed.
+
+Lemma hoare_app_fix : forall v1 v2 (f:var) x t1 H H' Q,
+  v1 = val_fix f x t1 ->
+  f <> x ->
+  pay_one H H' ->
+  hoare (subst x v2 (subst f v1 t1)) H' Q ->
+  hoare (trm_app v1 v2) H Q.
+Proof using.
+  introv E D HP M. intros h K0.
+  lets (h'&K'&->): pay_one_elim (rm HP) (rm K0).
+  forwards (n&h''&v&R1&K1&E1): (rm M) K'.
+  exists (n+1)%nat h'' v. splits*.
+  { applys* eval_app_fix_val. applys_eq R1; try fmap_eq. }
+  { rew_heap. math. }
+Qed.
+
+Lemma hoare_let : forall z t1 t2 H Q Q1,
+  hoare t1 H Q1 ->
+  (forall v, hoare (subst1 z v t2) (Q1 v) Q) ->
+  hoare (trm_let z t1 t2) H Q.
+Proof using.
+  introv M1 M2 Hh.
+  forwards* (n1&h1'&v1&R1&K1&E1): (rm M1).
+  forwards* (n2&h2'&v2&R2&K2&E2): (rm M2).
+  exists (n1+n2)%nat h2' v2. splits~.
+  { applys~ eval_let R2. }
+  { math. }
+Qed.
+
+Lemma hoare_if : forall (b:bool) t1 t2 H Q,
+  hoare (if b then t1 else t2) H Q ->
+  hoare (trm_if b t1 t2) H Q.
+Proof using.
+  introv M1. intros h Hh. forwards* (n1&h1'&v1&R1&K1&E1): (rm M1).
+  exists n1 h1' v1. splits*. { applys* eval_if. }
+Qed.
+
+Lemma hoare_ref : forall H v,
+  hoare (val_ref v)
+    H
+    (fun r => (\exists l, \[r = val_loc l] \* l ~~~> v) \* H).
+Proof using.
+  intros. intros h Hh.
+  forwards~ (l&Dl&Nl): (Fmap.single_fresh null (h^s) v).
+  forwards~ Hh1': hsingle_intro l v.
+  sets h1': ((Fmap.single l v),credits_zero).
+  exists 0%nat (h1' \u h) (val_loc l). splits~.
+  { applys~ eval_ref_sep. }
+  { apply~ hstar_intro. { exists l. xsimplh~. } }
+Qed.
+
+Lemma hoare_get : forall H v l,
+  hoare (val_get (val_loc l))
+    ((l ~~~> v) \* H)
+    (fun x => \[x = v] \* (l ~~~> v) \* H).
+Proof using.
+  intros. intros h Hh. exists 0%nat h v. splits~.
+  { destruct Hh as (h1&h2&(N1a&N1b)&N2&N3&N4).
+    subst h. applys* eval_get_sep. }
+  { xsimplh~. }
+Qed.
+
+Lemma hoare_set : forall H w l v,
+  hoare (val_set (val_loc l) w)
+    ((l ~~~> v) \* H)
+    (fun r => \[r = val_unit] \* (l ~~~> w) \* H).
+Proof using.
+  intros. intros h Hh. destruct Hh as (h1&h2&(N1a&N1b&N1c)&N2&N3&N4).
+  forwards~ Hh1': hsingle_intro l w.
+  sets h1': ((Fmap.single l w), credits_zero).
+  exists 0%nat (h1' \u h2) val_unit. splits~.
+  { subst h. applys eval_set_sep; rew_heap*. }
+  { rewrite hstar_hpure. split~.
+    { applys hstar_intro.
+      { hnfs~. }
+      { xsimplh~. }
+      { unfold h1'. unfolds heap_disjoint. rewrite N1a in N3.
+        applys~ Fmap.disjoint_single_set v. } } }
+   { subst h h1'. rew_heap. simpl. math. }
+Qed.
+
+Lemma hoare_free : forall H l v,
+  hoare (val_free (val_loc l))
+    ((l ~~~> v) \* H)
+    (fun r => \[r = val_unit] \* H).
+Proof using.
+  intros. intros h Hh. destruct Hh as (h1&h2&N1&N2&N3&N4).
+  lets (E1&X1): hsingle_inv N1.
+  exists 0%nat h2 val_unit. split.
+  { subst h h1. applys* eval_free_sep. }
+  { subst h h1. rewrite* hstar_hpure. }
+Qed.
+
+(* ---------------------------------------------------------------------- *)
+(* ** Definition of SL triples *)
+
 Definition triple (t:trm) (H:hprop) (Q:val->hprop) : Prop :=
   forall H', hoare t (H \* H') (Q \*+ H' \*+ \GC).
 
---------------
-heap = fmap loc (val * pourcentage)  (O,1]
-heap_state h = map (fun x (v,pour) => v) h
-heap_ro h = filter (fun x (v,pour) => pour < 1) h
+(** Triple satisfy the [local] predicate *)
 
-Definition hoare (t:trm) (H:hprop) (Q:val->hprop) :=
-  forall h, H h -> exists h' v, eval (heap_state h) t (heap_state h') v
-                             /\ Q v h'
-                             /\ h'^ro = h^ro.
+Lemma local_triple : forall t,
+  local (triple t).
+Proof using.
+  intros. applys local_intro. intros H Q M H'.
+  intros h (h1&h2&N1&N2&N3&N4). hnf in M.
+  lets (H1&H2&Q1&R): M N1.
+  rewrite <- hstar_assoc, hstar_comm, hstar_hpure in R.
+  lets ((R1&R2)&R3): R.
+  forwards (n&h'&v&S1&S2&S3): R1 (H2\*H') h.
+  { subst h. rewrite <- hstar_assoc. exists~ h1 h2. }
+  exists n h' v. splits~. rewrite <- hstar_hgc_hgc.
+  applys himpl_inv S2.
+  xchange (R2 v). xsimpl.
+Qed.
 
---------------
-
-heap = (state * state * disjoint (fst,snd))
-^rw : (f,r) -> (f,empty)
-^ro : (f,r) -> (empty,r)
-
-Definition hoare (t:trm) (H:hprop) (Q:val->hprop) :=
-  forall h, H h -> exists h' v, eval (heap_state h) t (heap_state h') v
-                             /\ Q v (h'^rw)
-                             /\ h'^ro = h^ro.
+Hint Resolve local_triple.
 
 
-Definition triple (t:trm) (H:hprop) (Q:val->hprop) : Prop :=
-  forall HI HO, isframe HI HO ->
-    hoare t (H \* HI) (Q \*+ HO \*+ \GC).
+(* ---------------------------------------------------------------------- *)
+(* ** Structural rules *)
 
+Lemma triple_conseq : forall t H' Q' H Q,
+  triple t H' Q' ->
+  H ==> H' ->
+  Q' ===> Q ->
+  triple t H Q.
+Proof using. intros. applys* local_conseq. Qed.
 
-Lemma triple_frame : forall HI HO t H1 Q1,
+Lemma triple_frame : forall t H Q H',
+  triple t H Q ->
+  triple t (H \* H') (Q \*+ H').
+Proof using. intros. applys* local_frame. Qed.
+
+Lemma triple_hgc_pre : forall t H Q,
+  triple t H Q ->
+  triple t (H \* \GC) Q.
+Proof using. intros. applys* local_hgc_pre. Qed.
+
+Lemma triple_hgc_post : forall t H Q,
+  triple t H (Q \*+ \GC) ->
+  triple t H Q.
+Proof using. intros. applys* local_hgc_post. Qed.
+
+Lemma triple_hexists : forall t (A:Type) (J:A->hprop) Q,
+  (forall x, triple t (J x) Q) ->
+  triple t (hexists J) Q.
+Proof using. intros. applys* local_hexists. Qed.
+
+Lemma triple_hforall : forall A (x:A) t (J:A->hprop) Q,
+  triple t (J x) Q ->
+  triple t (hforall J) Q.
+Proof using. intros. applys* local_hforall. Qed.
+
+Lemma triple_hpure : forall t (P:Prop) H Q,
+  (P -> triple t H Q) ->
+  triple t (\[P] \* H) Q.
+Proof using. intros. applys* local_hpure. Qed.
+
+Lemma triple_hwand_hpure_l : forall t (P:Prop) H Q,
+  P ->
+  triple t H Q ->
+  triple t (\[P] \-* H) Q.
+Proof using. intros. applys* local_hwand_hpure_l. Qed.
+
+Lemma triple_hor : forall t H1 H2 Q,
+  triple t H1 Q ->
+  triple t H2 Q ->
+  triple t (hor H1 H2) Q.
+Proof using. intros. applys* local_hor. Qed.
+
+Lemma triple_hand_l : forall t H1 H2 Q,
+  triple t H1 Q ->
+  triple t (hand H1 H2) Q.
+Proof using. intros. applys* local_hand_l. Qed.
+
+Lemma triple_hand_r : forall t H1 H2 Q,
+  triple t H2 Q ->
+  triple t (hand H1 H2) Q.
+Proof using. intros. applys* local_hand_r. Qed.
+
+Lemma triple_conseq_frame_hgc : forall H2 H1 Q1 t H Q,
   triple t H1 Q1 ->
-  isframe HI HO ->
-  triple t (H1 \* HI) (Q1 \*+ HO).
+  H ==> H1 \* H2 ->
+  Q1 \*+ H2 ===> Q \*+ \GC ->
+  triple t H Q.
+Proof using. intros. applys* local_conseq_frame_hgc. Qed.
 
-Definition onlyro (H:hprop) : Prop :=
-  forall h, H h -> h^rw = heap_empty.
 
-Definition onlyrw (H:hprop) : Prop :=
-  forall h, H h -> h^ro = heap_empty.
 
-Definition isframe (HI HO:hprop) : Prop :=
-  exists HR, onlyrw HO /\ onlyro HR /\ HI = HO \* HR.
+
+(* ---------------------------------------------------------------------- *)
+(* ** SL rules for terms *)
+
+Lemma triple_of_hoare : forall t H Q,
+  (forall H',
+     exists Q', hoare t (H \* H') Q' /\ Q' ===> Q \*+ H' \*+ \GC) ->
+  triple t H Q.
+Proof using.
+  introv M. intros H'. forwards* (Q'&R&W): M HF. applys* hoare_conseq R.
+Qed.
+
+Lemma triple_val : forall v,
+  triple (trm_val v) \[] (fun r => \[r = v]).
+Proof using.
+  intros. intros H' HF. rew_heaps.
+  applys hoare_conseq.
+  { applys* hoare_val. }
+  { xsimpl. }
+  { xsimpl*. }
+Qed.
+
+Lemma triple_val_framed : forall v H Q,
+  H ==> Q v ->
+  onlyrw H ->
+  triple (trm_val v) H Q.
+Proof using.
+  introv M N. applys triple_conseq_frame_onlyrw N.
+  { applys triple_val. }
+  { xsimpl. }
+  { xchanges M. intros ? ->. xsimpl*. }
+Qed.
+
+Lemma triple_fix : forall f x t1,
+  triple (trm_fix f x t1) \[] (fun r => \[r = (val_fix f x t1)]).
+Proof using.
+  intros. intros H'. rew_heaps.
+  applys hoare_conseq.
+  { applys* hoare_fix. }
+  { xsimpl. }
+  { xsimpl*. }
+Qed.
+
+Lemma triple_fix_framed : forall f x t1 H Q,
+  H ==> Q (val_fix f x t1) ->
+  onlyrw H ->
+  triple (trm_fix f x t1) H Q.
+Proof using.
+  introv M N. applys triple_conseq_frame_onlyrw N.
+  { applys triple_fix. }
+  { xsimpl. }
+  { xchanges M. intros ? ->. xsimpl*. }
+Qed.
+
+Lemma triple_let : forall (z:var) t1 t2 H1 H2 Q Q1,
+  triple t1 (H1 \* RO H2) Q1 ->
+  (forall v, triple (subst1 z v t2) (Q1 v \* H2) Q) ->
+  triple (trm_let z t1 t2) (H1 \* H2) Q.
+Proof using.
+  introv M1 M2.
+  applys triple_of_hoare. intros H'.
+  unfolds in M1.
+  esplit. split.
+  { applys hoare_conseq.
+    { applys hoare_let H1 H2 (Q1 \*+ \GC) (Q \*+ \GC) HF.
+      { applys hoare_conseq.
+        { applys M1 HF. } { xsimpl. } { xsimpl. } }
+      { intros v H3 N3. lets NO: onlyrw_of_isframe HF.
+        forwards* HFa: isframe_onlyrw (HO \* \GC) isframe_hempty.
+        { auto with onlyrw. }
+        forwards* HFb: isframe_onlyro H3 (rm HFa). rew_heaps in HFb.
+        applys hoare_conseq.
+        { applys M2 HFb. } { xsimpl. }
+        { xsimpl. } } }
+    { xsimpl. }
+    { xsimpl. } }
+  { xsimpl. }
+Qed.
+
+Lemma triple_if : forall (b:bool) t1 t2 H Q,
+  triple (if b then t1 else t2) H Q ->
+  triple (trm_if b t1 t2) H Q.
+Proof using.
+  introv M1. intros H'. applys hoare_if. applys~ M1.
+Qed.
+
+Lemma triple_app_fix : forall (f:var) F x X t1 H Q,
+  F = val_fix f x t1 ->
+  f <> x ->
+  pay_one H H' ->
+  triple (subst2 f F x X t1) H' Q ->
+  triple (trm_app F X) H Q.
+Proof using.
+  introv EF N M. intros H'. applys* hoare_app_fix EF N.
+Qed.
+
+Lemma triple_ref : forall v,
+  triple (val_ref v)
+    \[]
+    (fun r => \exists l, \[r = val_loc l] \* l ~~~> v).
+Proof using.
+  intros. applys~ triple_of_hoare.
+  intros H'. esplit. split.
+  { rew_heap. applys* hoare_ref HF. } { xsimpl*. }
+Qed.
+
+Lemma triple_get_ro : forall v l,
+  triple (val_get (val_loc l))
+    (RO (l ~~~> v))
+    (fun x => \[x = v]).
+Proof using.
+  intros. applys triple_of_hoare. intros H'.
+  esplit; split. { applys* hoare_get_ro. } { xsimpl*. }
+Qed.
+
+Lemma triple_set : forall (w:val) l v,
+  triple (val_set (val_loc l) w)
+    (l ~~~> v)
+    (fun r => \[r = val_unit] \* l ~~~> w).
+Proof using.
+  intros. applys triple_of_hoare. intros H'.
+  esplit; split. { applys* hoare_set. } { xsimpl*. }
+Qed.
+
+Lemma triple_set' : forall (w:val) l v,
+  triple (val_set (val_loc l) w)
+    (l ~~~> v)
+    (fun r => l ~~~> w).
+Proof using.
+  intros. applys triple_conseq.
+  { applys* triple_set. } { xsimpl*. } { xsimpl*. }
+Qed.
+
+Lemma triple_free : forall l v,
+  triple (val_free (val_loc l))
+    (l ~~~> v)
+    (fun r => \[r = val_unit]).
+Proof using.
+  intros. applys triple_of_hoare. intros H'.
+  esplit; split. { applys* hoare_free. } { xsimpl*. }
+Qed.
+
+
+
+(* ---------------------------------------------------------------------- *)
+(* ** Intrepretation for full executions *)
+
+(** Interpretation of triples for full executions:
+    the number of credits in the precondition is an upper bound
+    on the number of steps taken by the execution. *)
+
+Lemma triple_hcredits_haffine_post : forall t n Q,
+  triple t (\$ n) Q ->
+  exists n' n'' h v s',
+     eval n' Fmap.empty t s' v
+  /\ (Q v \* \GC) (s',n'')
+  /\ n'' >= 0
+  /\ ((n':int) <= n).
+Proof using.
+  introv M F. forwards (n'&h&v&R&K&C): (rm M) hempty (mk_heap_credits n).
+  { rew_heap. applys hcredits_mk_heap_credits. }
+  rew_heap in K. exists n' h v. splits*.
+  { simpls. forwards N: haffine_heap_inv K.
+    { applys haffine_hstar. applys* F. applys haffine_hgc. }
+   math. }
+Qed.
+
