theories/SepBase.v
@@ -638,16 +638,16 @@ Proof using.
   exists h2' v2. splits~. { applys~ eval_constr_trm R2. }
 Qed.
 
-Lemma hoare_let : forall z t1 t2 H Q Q1,
-  hoare t1 H Q1 ->
-  (forall v, hoare (subst1 z v t2) (Q1 v) Q) ->
-  hoare (trm_let z t1 t2) H Q.
-Proof using.
-  introv M1 M2 Hh.
-  forwards* (h1'&v1&R1&K1): (rm M1).
-  forwards* (h2'&v2&R2&K2): (rm M2).
-  exists h2' v2. splits~. { applys~ eval_let_trm R2. }
-Qed.
+  Lemma hoare_let : forall z t1 t2 H Q Q1,
+    hoare t1 H Q1 ->
+    (forall v, hoare (subst1 z v t2) (Q1 v) Q) ->
+    hoare (trm_let z t1 t2) H Q.
+  Proof using.
+    introv M1 M2 Hh.
+    forwards* (h1'&v1&R1&K1): (rm M1).
+    forwards* (h2'&v2&R2&K2): (rm M2).
+    exists h2' v2. splits~. { applys~ eval_let_trm R2. }
+  Qed.
 
 Lemma hoare_seq : forall t1 t2 H Q H1,
   hoare t1 H (fun r => H1) ->
