theories/SepFrac.v
@@ -1,0 +1,61 @@
+
+
+Definition hoare (t:trm) (H:hprop) (Q:val->hprop) :=
+  forall h, H h -> exists h' v, eval (heap_state h) t (heap_state h') v
+                             /\ Q v h'
+
+Definition triple (t:trm) (H:hprop) (Q:val->hprop) : Prop :=
+  forall H', hoare t (H \* H') (Q \*+ H' \*+ \GC).
+
+
+--------------
+heap = (state * Z)
+
+Definition hoare (t:trm) (H:hprop) (Q:val->hprop) :=
+  forall h, H h -> exists h' v, evaln n (heap_state h) t (heap_state h') v
+                             /\ Q v h'
+                             /\ heap_credits h = n + heap_credits h'.
+
+Definition triple (t:trm) (H:hprop) (Q:val->hprop) : Prop :=
+  forall H', hoare t (H \* H') (Q \*+ H' \*+ \GC).
+
+--------------
+heap = fmap loc (val * pourcentage)  (O,1]
+heap_state h = map (fun x (v,pour) => v) h
+heap_ro h = filter (fun x (v,pour) => pour < 1) h
+
+Definition hoare (t:trm) (H:hprop) (Q:val->hprop) :=
+  forall h, H h -> exists h' v, eval (heap_state h) t (heap_state h') v
+                             /\ Q v h'
+                             /\ h'^ro = h^ro.
+
+--------------
+
+heap = (state * state * disjoint (fst,snd))
+^rw : (f,r) -> (f,empty)
+^ro : (f,r) -> (empty,r)
+
+Definition hoare (t:trm) (H:hprop) (Q:val->hprop) :=
+  forall h, H h -> exists h' v, eval (heap_state h) t (heap_state h') v
+                             /\ Q v (h'^rw)
+                             /\ h'^ro = h^ro.
+
+
+Definition triple (t:trm) (H:hprop) (Q:val->hprop) : Prop :=
+  forall HI HO, isframe HI HO ->
+    hoare t (H \* HI) (Q \*+ HO \*+ \GC).
+
+
+Lemma triple_frame : forall HI HO t H1 Q1,
+  triple t H1 Q1 ->
+  isframe HI HO ->
+  triple t (H1 \* HI) (Q1 \*+ HO).
+
+Definition onlyro (H:hprop) : Prop :=
+  forall h, H h -> h^rw = heap_empty.
+
+Definition onlyrw (H:hprop) : Prop :=
+  forall h, H h -> h^ro = heap_empty.
+
+Definition isframe (HI HO:hprop) : Prop :=
+  exists HR, onlyrw HO /\ onlyro HR /\ HI = HO \* HR.
